{
 "cells": [
  {
   "cell_type": "markdown",
   "metadata": {},
   "source": [
    "Jireh M. Dominguez BSCS 1 Discrete Math 2 Group 3 Lecture 1\n",
    "\n",
    "### Question 1:\n",
    "**Proof by Contradiction:**\n",
    "\n",
    "1. **Assumption:** Let's assume for the sake of contradiction that Euler's number $e$ is rational, expressed as $e = \\frac{p}{q}$ where $p$ and $q$ are integers and $q \\neq 0$.\n",
    "\n",
    "2. **Recall the Definition of $e$:** Euler's number $e$ is defined as the sum of the series $\\sum_{k=0}^\\infty \\frac{1}{k!}$.\n",
    "\n",
    "3. **Partial Sum of the Series:** Consider the partial sum $S_n$ of the series up to $n$ terms: \n",
    "\\begin{equation*}\n",
    "S_n = \\frac{1}{0!} + \\frac{1}{1!} + \\frac{1}{2!} + \\ldots + \\frac{1}{n!}\n",
    "\\end{equation*}\n",
    "\n",
    "4. **Manipulation of Partial Sum:** We can express $q! \\cdot S_n$ as: \n",
    "\\begin{equation*}\n",
    "q! \\cdot S_n = q! \\cdot \\left(\\frac{1}{0!} + \\frac{1}{1!} + \\frac{1}{2!} + \\ldots + \\frac{1}{n!}\\right)\n",
    "\\end{equation*}\n",
    "\n",
    "5. **Expression Expansion:** This expands to: \n",
    "\\begin{equation*}\n",
    "q! \\cdot S_n = q! + \\frac{q!}{1!} + \\frac{q!}{2!} + \\ldots + \\frac{q!}{n!}\n",
    "\\end{equation*}\n",
    "\n",
    "6. **Contradiction:** However, $q! \\cdot S_n$ should be very close to $p$, but $p - q! \\cdot S_n$ results in a non-zero positive integer, contradicting the assumption that $e = \\frac{p}{q}$.\n",
    "\n",
    "7. **Conclusion:** Thus, Euler's number $e$ cannot be rational, implying $e \\notin \\mathbb{Q}$.\n",
    "\n",
    "### Question 2:\n",
    "**Minkowski's Inequality Proof:**\n",
    "1. Use of Holder's Inequality: Start with Holder's Inequality:\n",
    "\\begin{equation*}\n",
    "\\sum_{k=1}^n |a_k b_k| \\leq \\left( \\sum_{k=1}^n |a_k|^p \\right)^{\\frac{1}{p}} \\left( \\sum_{k=1}^n |b_k|^q \\right)^{\\frac{1}{q}}\n",
    "\\end{equation*}\n",
    "\n",
    "2. Definition of Variables: Define $a_k = |x_k|^p$ and $b_k = |y_k|^p$.\n",
    "\n",
    "3. Application of Holder's Inequality: Apply Holder's Inequality with the new definitions:\n",
    "\\begin{equation*}\n",
    "\\sum_{k=1}^n |x_k y_k|^p \\leq \\left( \\sum_{k=1}^n |x_k|^p \\right)^{\\frac{1}{p}} \\left( \\sum_{k=1}^n |y_k|^q \\right)^{\\frac{1}{q}}\n",
    "\\end{equation*}\n",
    "\n",
    "4. Take the $p$-th Root: Take the $p$-th root of both sides:\n",
    "\\begin{equation*}\n",
    "\\left( \\sum_{k=1}^n |x_k y_k|^p \\right)^{\\frac{1}{p}} \\leq \\left( \\sum_{k=1}^n |x_k|^p \\right)^{\\frac{1}{p}} \\left( \\sum_{k=1}^n |y_k|^p \\right)^{\\frac{1}{q}}\n",
    "\\end{equation*}\n",
    "\n",
    "5. Use of Relationship between $p$ and $q$: Recognize that $\\frac{p-1}{p} = 1 - \\frac{1}{p}$.\n",
    "\n",
    "6. Apply Holder's Inequality Again: Apply Holder's Inequality to eliminate the $\\frac{p-1}{p}$ term:\n",
    "\\begin{equation*}\n",
    "\\left( \\sum_{k=1}^n |y_k|^p \\right)^{\\frac{p-1}{p}} \\leq n^{\\frac{p-1}{p}} \\left( \\sum_{k=1}^n |y_k|^p \\right)^{\\frac{1}{p}}\n",
    "\\end{equation*}\n",
    "\n",
    "7. Substitute Back into the Inequality: Substitute this equation back into the inequality:\n",
    "\\begin{equation*}\n",
    "\\left( \\sum_{k=1}^n |x_k + y_k|^p \\right)^{\\frac{1}{p}} \\leq n^{\\frac{1}{p}} \\left( \\sum_{k=1}^n |x_k|^p \\right)^{\\frac{1}{p}} \\left( \\sum_{k=1}^n |y_k|^p \\right)^{\\frac{1}{p}}\n",
    "\\end{equation*}\n",
    "\n",
    "\n",
    "### Question 3:\n",
    "**Triangle Inequality Proof:**\n",
    "\n",
    "1. **Absolute Value Definition:** We define the absolute value of a real number $x$ as: \n",
    "\\begin{equation*}\n",
    "|x| = \\begin{cases} x, & \\text{if } x \\geq 0 \\\\ -x, & \\text{if } x < 0 \\end{cases}\n",
    "\\end{equation*}\n",
    "\n",
    "2. **Case Analysis:** We consider four cases based on the signs of $x$ and $y$.\n",
    "\n",
    "3. **Case 1:** When $x \\geq 0$ and $y \\geq 0$, it directly follows that: \n",
    "\\begin{equation*}\n",
    "|x + y| = x + y \\leq |x| + |y|\n",
    "\\end{equation*}\n",
    "\n",
    "4. **Case 2:** Similarly, when $x < 0$ and $y < 0$, we have: \n",
    "\\begin{equation*}\n",
    "|x + y| = -(x + y) = -x - y \\leq |x| + |y|\n",
    "\\end{equation*}\n",
    "\n",
    "5. **Case 3:** For $x \\geq 0$ and $y < 0$, we show that: \n",
    "\\begin{equation*}\n",
    "|x + y| \\leq |x| - y\n",
    "\\end{equation*}\n",
    "\n",
    "6. **Case 4:** Similarly, when $x < 0$ and $y \\geq 0$, we have: \n",
    "\\begin{equation*}\n",
    "|x + y| \\leq -x + |y|\n",
    "\\end{equation*}\n",
    "\n",
    "7. **Conclusion:** In all cases, we establish: \n",
    "\\begin{equation*}\n",
    "|x + y| \\leq |x| + |y|\n",
    "\\end{equation*}, thus proving the triangle inequality.\n",
    "\n",
    "### Question 4:\n",
    "**Sedrakayan's Lemma Proof:**\n",
    "\n",
    "1. Use of Cauchy-Schwarz Inequality: We begin by invoking the Cauchy-Schwarz Inequality:\n",
    "\\begin{equation*}\n",
    "\\left(\\sum_{i=1}^n u_i v_i\\right)^2 \\leq \\left(\\sum_{i=1}^n u_i^2\\right) \\left(\\sum_{i=1}^n v_i^2\\right)\n",
    "\\end{equation*}\n",
    "\n",
    "2. Definition of Variables: Define $\\mathbf{u} = (u_1, u_2, ..., u_n)$ and $\\mathbf{v} = (\\sqrt{v_1}, \\sqrt{v_2}, ..., \\sqrt{v_n})$.\n",
    "\n",
    "3. Application of Cauchy-Schwarz: Apply Cauchy-Schwarz Inequality to the vectors $\\mathbf{u}$ and $\\mathbf{v}$:\n",
    "\\begin{equation*}\n",
    "\\left(\\sum_{i=1}^n u_i \\sqrt{v_i}\\right)^2 \\leq \\left(\\sum_{i=1}^n u_i^2\\right) \\left(\\sum_{i=1}^n v_i\\right)\n",
    "\\end{equation*}\n",
    "\n",
    "4. Rearrangement: Rearrange the inequality:\n",
    "\\begin{equation*}\n",
    "\\frac{\\left(\\sum_{i=1}^n u_i\\right)^2}{\\sum_{i=1}^n v_i} \\leq \\sum_{i=1}^n \\frac{u_i^2}{v_i}\n",
    "\\end{equation*}\n",
    "\n",
    "5. Conclusion: Sedrakayan's Lemma is established, affirming that for any positive real numbers $u_i$ and $v_i$:\n",
    "\\begin{equation*}\n",
    "\\frac{\\left(\\sum_{i=1}^n u_i\\right)^2}{\\sum_{i=1}^n v_i} \\leq \\sum_{i=1}^n \\frac{u_i^2}{v_i}\n",
    "\\end{equation*}"
   ]
  }
 ],
 "metadata": {
  "language_info": {
   "name": "python"
  }
 },
 "nbformat": 4,
 "nbformat_minor": 2
}
